\begin{align}
\begin{split}
\label{eq:full_model}
	 \mu &= \frac{m_{aa}}{m_p(\mu)} \nu(s) \phi_b(\mu,r,s) \phi_t r_t(m_r) \\
	 r &= \frac{\phi_t r_t(m_r)}{1+J_{sum}(\mu,r,s)} \\
	 \dot m_r &= \left[m_p(\mu) \frac{N_r J_r(\mu,r,s)}{J_{sum}(\mu,r,s)} - m_r \right] \mu \\
	 \dot m_{nr} &= \left[m_p(\mu) \frac{N_{nr} J_{nr}(\mu,r,s)}{J_{sum}(\mu,r,s)} - m_{nr}\right] \mu \\
	 \dot m_A &= \left[m_p(\mu) \frac{N_A J_A(\mu,r,s)}{J_{sum}(\mu,r,s)} - m_A \right] \mu \\
	 \dot V &= F_{in} - F_{out} \\
	 \dot n &= \mu n - \frac{F_{in}}{V} n \\
	 \dot s &= \frac{F_{in}}{V} (s_{feed} - s) - y^{-1} \mu x(n,\mu) 
\end{split}
\end{align}
